Koit.lean
@@ -13,6 +13,7 @@ import Koit.Facts.Domain
 import Koit.Facts.Facts
 import Koit.Facts.Smt
 import Koit.Facts.Entail
+import Koit.Effects.Effects
 import Koit.Check.Diag
 import Koit.Check.Env
 import Koit.Check.Types
